proof/correctness/avx2/KyberPolyvec_avx2_proof.ec
@@ -296,7 +296,8 @@ proof.
       rewrite Array768.initiE /=; first by move : (nttunpack_inbounds (k-512)) => /#.
       have ->: !(0 <= 512 + nttunpack_idx.[k - 512] && 512 + nttunpack_idx.[k - 512] < 256). move : nttunpack_inbounds => /#.
       have -> /=: !(256 <= 512 + nttunpack_idx.[k - 512] && 512 + nttunpack_idx.[k - 512] < 512). move : nttunpack_inbounds => /#.
-      admit. (* FIXME: use nttunpackK *)
+      rewrite mapiE 1:(nttunpack_inbounds (k-512)) 1:/# /nttpack initiE 1:(nttunpack_inbounds (k-512)) 1:/# /=.
+      move : nttpack_idxK; rewrite allP /= => ->. rewrite mem_iota -andabP; move : kbb kb => /#. trivial.
     case ( 256 <= k && k < 512).
     + move => kbb nkbb; rewrite (_: 0<= k <256 = false) 1:/# /=.
       rewrite /subarray256 => />.
@@ -304,14 +305,16 @@ proof.
       rewrite Array768.initiE /=; first by move : (nttunpack_inbounds (k-256)) => /#.
       have ->: !(0 <= 256 + nttunpack_idx.[k - 256] && 256 + nttunpack_idx.[k - 256] < 256). move : nttunpack_inbounds => /#.
       have -> /=: (256 <= 256 + nttunpack_idx.[k - 256] && 256 + nttunpack_idx.[k - 256] < 512). move : nttunpack_inbounds => /#.
-      admit. (* FIXME: use nttunpackK *)
-    + move => nkbb nkbbb; rewrite initiE 1:/# (_: 0<= k <256 = true) 1:/# /=.
+      rewrite mapiE 1:(nttunpack_inbounds (k-256)) 1:/# /nttpack initiE 1:(nttunpack_inbounds (k-256)) 1:/# /=.
+      move : nttpack_idxK; rewrite allP /= => ->. rewrite mem_iota -andabP; move : kbb kb => /#. trivial.
+    + move => nkbb nkbbb; rewrite initiE 1:/# (_: 0<= k < 256 = true) 1:/# /= (_: 0<= k < 256 = true) 1:/# /=.
       rewrite /subarray256 => />.
-      rewrite  /nttunpack initiE 1:/# //= initiE 1:(nttunpack_inbounds (k)) 1:/# /=.
-      rewrite Array768.initiE /=; first by move : (nttunpack_inbounds (k)) => /#.
+      rewrite  /nttunpack initiE 1:/# //= initiE 1:(nttunpack_inbounds k) 1:/# /=.
+      rewrite Array768.initiE /=; first by move : (nttunpack_inbounds k) => /#.
       rewrite (nttunpack_inbounds k) 1:/# /=.
-      admit. (* FIXME: use nttunpackK *)
-
+      rewrite mapiE 1:(nttunpack_inbounds k) 1:/# /nttpack initiE 1:(nttunpack_inbounds k) 1:/# /=.
+      move : nttpack_idxK; rewrite allP /= => ->. rewrite mem_iota -andabP; move : nkbb nkbbb kb => /#. trivial.
+     
   move => k kb; rewrite initiE 1:/# /=.
   case ( 512 <= k && k < 768);1: by smt(). 
   case ( 256 <= k && k < 512). 
@@ -380,6 +383,98 @@ proof.
   auto => />.
 qed.
 
+lemma polyvec_tobytes_corr mem _p _a:
+    equiv [ Mprevec.polyvec_tobytes ~ EncDec_AVX2.encode12_opt_vec :
+            pos_bound768_cxq a{1} 0 768 2 /\
+            lift_array768 (nttpackv a{1}) = _a /\
+            (forall i, 0<=i<768 => 0 <= a{2}.[i] <q) /\
+            map inFq a{2} = _a /\  valid_ptr _p (3*384) /\
+            Glob.mem{1} = mem /\ to_uint rp{1} = _p
+             ==>
+            touches mem Glob.mem{1} _p (3*384) /\
+            load_array1152 Glob.mem{1} _p = res{2}
+            ].
+proof.
+  proc => /=.
+  wp;ecall (KyberPolyAVX.poly_tobytes_corr (lift_array256 (nttpack (Array256.init (fun (i : int) => a{1}.[2 * 256 + i])))) (to_uint pp{1}) Glob.mem{1}).
+  wp;ecall (KyberPolyAVX.poly_tobytes_corr (lift_array256 (nttpack (Array256.init (fun (i : int) => a{1}.[256 + i])))) (to_uint pp{1}) Glob.mem{1}).
+  wp;ecall (KyberPolyAVX.poly_tobytes_corr (lift_array256 (nttpack (Array256.init (fun (i : int) => a{1}.[i])))) (to_uint pp{1}) Glob.mem{1}).
+
+  auto => /> &1 &2; rewrite /pos_bound768_cxq /pos_bound256_cxq /lift_array256 /lift_array768 /subarray256 !tP.
+  move => bnda1 bnda2 vals pbl pbh.
+
+  split.
+  + do split; 1,2: by move => *; rewrite initiE /=; smt().
+    + move => i ib; rewrite !mapiE // !initiE //=. move : (vals i); rewrite mapiE 1:/# mapiE 1:/# /=.
+      have -> /=: (0 <= i < 768). by move : ib => /#.
+      move => ->.
+      rewrite /nttpackv initiE 1:/# /= ib /= /subarray256 //=.
+    + move : pbh => /#.
+
+  rewrite /touches;move => ????????touch0; split.
+
+  + do split; 1: by  move => *; rewrite !initiE 1:/# /= !initiE  /#.
+    + by move => *; rewrite initiE /=; smt().
+    + rewrite tP => i ib; rewrite !mapiE // !initiE //=.
+      move : (vals (256 + i)); rewrite mapiE 1:/# mapiE 1:/# /=.
+      have -> /=: (0 <= 256 + i < 768). by move : ib => /#.
+      move => ->.
+      rewrite /nttpackv initiE 1:/# /=.
+      have ->: !(0 <= 256 + i && 256 + i < 256). by move : ib => /#.
+      have -> /=: (256 <= 256 + i && 256 + i < 512). by move : ib => /#.
+      congr. congr. move : i ib; rewrite -tP. rewrite pack_ext_eq tP => i ib.
+      rewrite initiE 1:/# /= initiE 1:/# /= initiE 1:/# /=.
+      have -> //=: !(0 <= 256 + i && 256 + i < 256). by move : ib => /#.
+    + by rewrite to_uintD_small; smt().
+    by rewrite to_uintD_small; smt().
+
+  rewrite /touches;move => ????????touch1; split. 
+
+  + do split; 1: by move => *; rewrite !initiE 1:/# /= !initiE 1:/# /= !initiE  /=  /#.
+    + by move => *; rewrite initiE /=; smt().
+    + rewrite tP => i ib; rewrite !mapiE // !initiE //=.
+      move : (vals (512 + i)); rewrite mapiE 1:/# mapiE 1:/# /=.
+      have -> /=: (0 <= 512 + i < 768). by move : ib => /#.
+      move => ->.
+      rewrite /nttpackv initiE 1:/# /=.
+      have ->: !(0 <= 512 + i && 512 + i < 256). by move : ib => /#.
+      have -> /=: !(256 <= 512 + i && 512 + i < 512). by move : ib => /#.
+      congr. congr. move : i ib; rewrite -tP. rewrite pack_ext_eq tP => i ib.
+      rewrite initiE 1:/# /= initiE 1:/# /= initiE 1:/# /= initiE 1:/# /=.
+      have ->: !(0 <= 512 + i && 512 + i < 256). by move : ib => /#.
+      have -> //=: !(256 <= 512 + i && 512 + i < 512). by move : ib => /#.
+    + by rewrite to_uintD_small; smt().
+    by rewrite to_uintD_small; smt().
+
+  rewrite /touches;move => ????????touch2.
+
+  do split. 
+  + move => k kb; move : (touch0 k _) (touch1 (k - 384) _) (touch2 (k - 768) _); 1..7: smt(). 
+    by rewrite !to_uintD_small /= /#.
+
+  rewrite /load_array1152 /fromarray384 /load_array384 tP => k kb; rewrite !initiE //=.
+  case (0 <= k < 384).
+  + move => kbb;  rewrite Array384.initiE //=.
+    move : (touch2 (k - 768) _); 1:smt(). 
+    rewrite to_uintD_small /=; 1: smt().
+    rewrite (_: to_uint rp{1} + 768 + (k - 768) = to_uint rp{1} + k);1 : by ring.
+    move => ->.
+    move : (touch1 (k - 384) _); 1:smt(). 
+    rewrite to_uintD_small /=; 1: smt().
+    by rewrite (_: to_uint rp{1} + 384 + (k - 384) = to_uint rp{1} + k);1 : by ring.
+
+  move=> nkb.
+  case (384 <= k < 768).
+  + move => kbb;  rewrite Array384.initiE 1:/# /=.
+    move : (touch2 (k - 768) _); 1:smt(). 
+    rewrite !to_uintD_small /=; 1,2: smt().
+    rewrite (_: to_uint rp{1} + 768 + (k - 768) = to_uint rp{1} + k);1 : by ring.
+    by rewrite (_: to_uint rp{1} + 384 + (k - 384) = to_uint rp{1} + k);1 : by ring.
+
+  + move => kbb;  rewrite Array384.initiE 1:/# /=.
+    rewrite !to_uintD_small /=; 1: smt().
+    by rewrite (_: to_uint rp{1} + 768 + (k - 768) = to_uint rp{1} + k);1 : by ring.
+qed.
 
 lemma polyvec_tobytes_equiv :
     equiv [ Jkem_avx2.M.__polyvec_tobytes ~ Jkem.M.__polyvec_tobytes :
@@ -387,7 +482,59 @@ lemma polyvec_tobytes_equiv :
              pos_bound768_cxq a{2} 0 768 2 /\
              lift_array768 a{1} = nttunpackv (lift_array768 a{2}) /\ ={rp,Glob.mem} ==> ={Glob.mem} ].
 proof.
-admitted. (* Miguel *)
+  transitivity Mprevec.polyvec_tobytes
+               (={rp, a, Glob.mem} ==> ={res, Glob.mem})
+               (pos_bound768_cxq a{1} 0 768 2 /\
+                pos_bound768_cxq a{2} 0 768 2 /\
+                lift_array768 a{1} = nttunpackv (lift_array768 a{2}) /\ ={rp,Glob.mem} ==>
+                ={Glob.mem}); first 2 by smt().
+    + symmetry. proc * => /=. call prevec_eq_polyvec_tobytes => //=.
+  transitivity EncDec_AVX2.encode12_opt_vec
+               (pos_bound768_cxq a{1} 0 768 2 /\ (forall i, 0<=i<768 => 0 <= a{2}.[i] < q) /\
+                map inFq a{2} = lift_array768 (nttpackv a{1}) /\ valid_ptr (to_uint rp{1}) (3*384) /\
+                ={Glob.mem} ==>
+                touches mem Glob.mem{1} (to_uint rp{1}) (3*384) /\
+                load_array1152 Glob.mem{1} (to_uint rp{1}) = res{2})
+               (pos_bound768_cxq a{2} 0 768 2 /\ (forall i, 0<=i<768 => 0 <= a{1}.[i] < q) /\
+                map inFq a{1} = lift_array768 a{2} /\ valid_ptr (to_uint rp{2}) (3*384) /\
+                ={Glob.mem} ==> ={Glob.mem}).
+               auto => &1 &2 />.
+                 exists Glob.mem{2}.
+                   exists (load_array1152 Glob.mem{2} (to_uint ap{2})).
+                     + auto => />.
+                     + admit. (* FIXME: bound on ap in pre-condition ?? *)
+               auto => &1 &2 &m [#] H0 H1 H2 [#] H3 H4 H5 />.
+                 rewrite nttunpackv_lift /lift_array768 Array768.tP => i i_bnds.
+                 rewrite mapiE 1:i_bnds /= mapiE 1:i_bnds /=. congr.
+                 rewrite -mapiE 1:i_bnds -(Array768.mapiE W16.to_sint _) 1:i_bnds.
+                 move : i i_bnds. rewrite -tP.
+                 rewrite H0 H3.
+                 rewrite nttunpackv_mapsint //=.
+    + proc * => /=.
+      ecall (polyvec_frombytes_corr (Glob.mem{1}) (to_uint ap{1})) => //=.
+  symmetry.
+  transitivity EncDec.decode12_vec
+               (valid_ptr (to_uint ap{1}) (3*384) /\ ={Glob.mem} /\ load_array1152 Glob.mem{1} (to_uint ap{1}) = a{2} ==>
+                map W16.to_sint res{1} = res{2}  /\
+                pos_bound768_cxq res{1} 0 768 2 /\
+                ={Glob.mem})
+                (={Glob.mem} /\ a{1} = a{2} ==>
+                res{1} = res{2} /\
+                ={Glob.mem}).
+               auto => &1 &2 [#] ap_bnds mem_eq load_def />.
+               exists Glob.mem{1}.
+               exists (load_array1152 Glob.mem{1} (to_uint ap{1})).
+               split.
+                 trivial.
+                 by rewrite mem_eq load_def.
+               auto => />.
+    + proc * => /=.
+      ecall (KyberPolyVec.polyvec_frombytes_corr (Glob.mem{1}) (to_uint ap{1})) => //=.
+  symmetry.
+  proc * => /=.
+  call decode12_opt_vec_corr.
+  auto => />.
+qed.
 
 
 lemma polyvec_add2_equiv  (ab bb : int):
